%\iffalse
\let\negmedspace\undefined
\let\negthickspace\undefined
\documentclass[journal,12pt,twocolumn]{IEEEtran}
\usepackage{cite}
\usepackage{amsmath,amssymb,amsfonts,amsthm}
\usepackage{algorithmic}
\usepackage{textcomp}
\usepackage{xcolor}
\usepackage{txfonts}
\usepackage{listings}
\usepackage{enumitem}
\usepackage{mathtools}
\usepackage{gensymb}
\usepackage{comment}
\usepackage[breaklinks=true]{hyperref}
\usepackage{tkz-euclide} 
\usepackage{listings}
\usepackage{gvv}                            \usepackage{tikz}
\usepackage{circuitikz}
\def\inputGnumericTable{}                                
\usepackage[latin1]{inputenc}                            
\usepackage{color}                                       
\usepackage{array}                                       
\usepackage{longtable}                                   
\usepackage{calc}                              
\usepackage{tikz}
\usepackage{multirow}                                    
\usepackage{hhline}                                      
\usepackage{ifthen}                            
\usepackage{caption}
\usepackage{lscape}
\usepackage{amsmath}
\newtheorem{theorem}{Theorem}[section]
\newtheorem{problem}{Problem}
\newtheorem{proposition}{Proposition}[section]
\newtheorem{lemma}{Lemma}[section]
\newtheorem{corollary}[theorem]{Corollary}
\newtheorem{example}{Example}[section]
\newtheorem{definition}[problem]{Definition}
\newcommand{\BEQA}{\begin{eqnarray}}
\newcommand{\EEQA}{\end{eqnarray}}
\newcommand{\define}{\stackrel{\triangle}{=}}
\theoremstyle{remark}
\newtheorem{rem}{Remark}

\begin{document}

\bibliographystyle{IEEEtran}
\vspace{3cm}

\title{GATE 2021 EE.20}
\author{EE23BTECH11010 - VENKATESH BANDAWAR$^{*}$% <-this % stops a space
}
\maketitle
\newpage
\bigskip

\section{Laplace Transform}
Laplace transform of integrals:\\
Let the function defined as $y(t) = \int_0^t f(u) du$ for all $t > 0$\\
Laplace transform of y(t) in t 
\begin{align}
    \mathcal{L} \brak{y(t)} &= \int_0^{\infty} e^{-st} y(t) dt\\
    &= \int_0^{\infty} e^{-st} \int_0^t f(u) du dt\\
    &= \int_0^t f(u) du \sbrak{- \frac{e^{-st}}{s}}_0^{\infty} + \int_0^{\infty} \frac{e^{-st}}{s} f(t) dt\\
    &= \frac{F(s)}{s}
\end{align}


\section{RLC Low Pass Filter}
\begin{figure}[!ht]
    \centering
    \input{figs/tikz1}
    \caption{RLC Low pass filter}
\end{figure}
\begin{table}[!ht]
    \centering
    \input{tables/table1}
    \caption{Input Parameters}
\end{table}
\begin{align}
    Y(s) &= I(s)Z_C\\
    &= \frac{X(s)}{Z_L + Z_R + Z_C}Z_C\\
    H(s) &= \frac{Y(s)}{X(s)}\\
    &= \frac{Z_C}{Z_L + Z_R + Z_C}\\
    &= \frac{\frac{1}{sC}}{sL + R + \frac{1}{sC}}\\
    &= \frac{1}{s^2LC + sRC + 1}\\
    \implies H(s) &= \omega_0^2\frac{1}{(s-p_1)(s-p_2)}
\end{align}
where,
\begin{align}
    \omega_0 &= \frac{1}{\sqrt{LC}}\\
    p_{1, 2} &= -\frac{R}{2L} \pm \sqrt{\brak{\frac{R}{2L}}^2 - \frac{1}{LC}}\\
    &= -\alpha \pm \sqrt{\alpha^2 - \omega_0^2}
\end{align}
where
\begin{align}
    \alpha &= \frac{R}{2L}
\end{align}
Damping Factor is given by,
\begin{align}
   \zeta &= \frac{\alpha}{\omega_0}\\
   &= \frac{R}{2}\sqrt{\frac{C}{L}}
\end{align}
\begin{table}[!ht]
    \centering
    \input{tables/table2}
    \caption{Effect of Damping Coefficient $\zeta$ on system behaviour}
\end{table}
\newpage
\begin{enumerate}
\item Overdamped Response
\begin{align}
    Y(s) &= X(s)H(s)\\
    &= \omega_0^2\frac{1}{s(s-p_1)(s-p_2)}\\
    &= \frac{c_0}{s} + \frac{c_1}{s-p_1} + \frac{c_2}{s-p_2}
\end{align}
where,
\begin{align}
    c_0 &= 1\\
    c_1 &= \frac{p_2}{p_1 - p_2}\\
    c_2 &= \frac{p_1}{p_2 - p_1}
\end{align}
Taking inverse Laplace,
\begin{align}
    y(t) &= c_0 + c_1e^{p_1t} + c_2e^{p_2t}\\
    &= \brak{1 + \frac{p_2}{p_1 - p_2}e^{p_1t} +  \frac{p_1}{p_2 - p_1}e^{p_2t}}u(t)
\end{align}

\begin{figure}[!ht]
    \centering
    \input{figs/tikz2}
    \caption{s-Plane for Overdamped case}
\end{figure}

\item Critically Damped Response
\begin{align}
    Y(s)&=X(s)H(s)\\
    &= \omega_0^2\frac{1}{s(s-p)^2}\\
    &= \frac{c_0}{s}+\frac{c_1}{\left(s-p\right)^2}+\frac{c_2}{s-p}
\end{align}
where
\begin{align}
    c_0 &= 1\\
    c_1 &= p\\
    c_2 &= -1
\end{align}
Taking Inverse Laplace,
\begin{align}
    y(t) &= c_0+(c_1t+c_2)e^{pt}\\
    &= \brak{1+(pt-1)e^{pt}}u(t)
\end{align}
\begin{figure}[!ht]
    \centering
    \input{figs/tikz3}
    \caption{s-Plane for Critically damped case}
\end{figure}

\item Underdamped Response
\begin{align}
    Y(s) &= X(s)H(s)\\
    &= \omega_0^2\frac{1}{s(s-p)(s-p^\ast)}\\
    &= \frac{c_0}{s}+\frac{c_1}{s-p}+\frac{c_2}{s-p^\ast}
\end{align}
where,
\begin{align}
    c_0 &= 1\\
    c_1 &= \frac{p^\ast}{p-p^\ast}\\
    c_2 &= \frac{p}{p^\ast-p}
\end{align}
Taking Inverse Laplace,
\begin{align}
    y(t) &= c_0+c_1e^{pt}+c_2e^{p^\ast t}\\
    &= 1+\frac{\abs{p}}{\omega_d}\ e^{-\sigma t}\frac{
    e^{j(\omega_d t+\varphi)}+e^{-j(\omega_d t+\varphi)}}{2}\\
    &= \brak{1+\frac{|p|}{\omega_d}e^{-\sigma t}\cos(\omega_d t+\varphi)}u(t)
\end{align}
where,
\begin{align}
    \abs{p}&=\sqrt{{\omega_d}^2+\sigma^2}\\
    \omega_d&=\omega_0\sqrt{1-\zeta^2}\\
    \sigma&=\omega_0\zeta\\
    \varphi&=\pi-\tan^{-1}\frac{\sigma}{\omega_d}
\end{align}
\begin{figure}[!ht]
    \centering
    \input{figs/tikz4}
    \caption{s-Plane for Under damped case}
\end{figure}
\end{enumerate}
\begin{figure}
    \centering
    \includegraphics[width = \columnwidth]{figs/plot.png}
    \caption{Plot of y(t) in all three cases}
\end{figure}
\end{document}
